ulib/LowStar.RST.Array.fst
@@ -15,8 +15,6 @@
 *)
 module LowStar.RST.Array
 
-friend LowStar.Array
-
 let index (#a:Type) (b:A.array a) (i:UInt32.t) = reveal_array(); A.index b i
 
 let upd (#a:Type) (b:A.array a) (i:UInt32.t) (v:a) =
@@ -36,7 +34,7 @@ let upd (#a:Type) (b:A.array a) (i:UInt32.t) (v:a) =
   (**) same_perm_seq_always_constant h0 h1 b
 
 let alloc (#a:Type) (init:a) (len:UInt32.t) =
-  (**) reveal_array();
+  (**) reveal_full_array();
   (**) reveal_rst_inv();
   (**) reveal_modifies();
   let b = A.alloc init len in
@@ -46,7 +44,7 @@ let alloc (#a:Type) (init:a) (len:UInt32.t) =
   b
 
 let free (#a:Type) (b:A.array a) =
-  (**) reveal_array();
+  (**) reveal_full_array();
   (**) reveal_empty_resource();
   (**) reveal_rst_inv();
   (**) reveal_modifies();
@@ -122,142 +120,27 @@ let glue #a b b1 b2 =
 
 #pop-options
 
-
-
-abstract
-let full_array_view (#a:Type) (b:A.array a) : view (varray a) =
-  reveal_view ();
-  let fp = Ghost.hide (A.loc_freed_mreference b.A.content) in
-  let inv h =
-    A.live h b /\ constant_perm_seq h b
-  in
-  let sel (h: HS.mem) : GTot (varray a) = { s = A.as_seq h b; p = A.get_perm h b 0 } in
-  {
-    fp = fp;
-    inv = inv;
-    sel = sel
-  }
-
-
-let full_array_resource (#a:Type) (b:A.array a) =
-  as_resource (full_array_view b)
-
-let promote (#a:Type) (b:A.array a) : RST unit
-  (full_array_resource b)
-  (fun _ -> array_resource b)
-  (fun _ -> True)
-  (fun _ _ _ -> True)
-  = 
-  let h0 = HST.get() in
-  reveal_array();
-  reveal_rst_inv();
-  reveal_modifies();
-  // assume     (forall frame .
-  //     A.loc_disjoint frame (A.loc_array b) /\
-  //     A.loc_includes (A.loc_not_unused_in h0) frame
-  //     ==>
-  //     A.loc_disjoint frame (A.loc_freed_mreference b.A.content) /\
-  //     A.loc_includes (A.loc_not_unused_in h0) frame);
-
-//  assume (modifies (array_resource b) (full_array_resource b) h0 h0);
-  ()
-
-let test (#a:Type) (b:A.array a) (v:a): RST unit
-  (full_array_resource b)
-  (fun _ -> full_array_resource b)
-  (fun h0 -> P.allows_write (sel (full_array_view b) h0).p)
-  (fun _ _ _ -> True)
-  =
-  reveal_array();
-  reveal_rst_inv();
-  reveal_modifies();
-  upd b 0ul v;
-  ()
-
-assume
-val arr_free (#a: Type) (b: A.array a) : HST.ST unit
-  (requires (fun h0 -> A.writeable h0 b /\ A.live  h0 b /\ A.freeable b))
-  (ensures (fun h0 _ h1 ->
-    Map.domain (HS.get_hmap h1) `Set.equal` Map.domain (HS.get_hmap h0) /\
-    (HS.get_tip h1) == (HS.get_tip h0) /\
-    A.modifies (A.loc_freed_mreference b.A.content) h0 h1 /\
-    HS.live_region h1 (A.frameOf b)
-  ))
-
-let full_free (#a:Type) (b:A.array a)
-  : RST unit (full_array_resource b)
-             (fun _ -> empty_resource)
-             (fun h0 -> A.freeable b /\ P.allows_write (sel (array_view b) h0).p)
-             (fun _ _ _ -> True)
-  =  (**) reveal_array();
-  (**) reveal_empty_resource();
-  (**) reveal_rst_inv();
-  (**) reveal_modifies();
-  arr_free b
-
-val arr_alloc (#a:Type0) (init:a) (len:UInt32.t)
-  : ST (A.array a)
-       (requires fun _ -> UInt32.v len > 0)
-       (ensures fun h0 b h1 ->
-         A.modifies A.loc_none h0 h1 /\
-         A.fresh_loc (A.loc_freed_mreference b.A.content) h0 h1 /\
-         A.writeable h1 b /\
-         A.freeable b /\
-         A.as_seq h1 b == Seq.create (UInt32.v len) init)
-
-let arr_alloc #a init len =
-  let perm_map_pid = Ghost.hide (
-    let (vp, pid) = LowStar.Permissions.new_value_perms init true in
-    ((vp <: LowStar.Permissions.perms_rec a), Ghost.hide pid)
-  ) in
-  let v = (init, Ghost.hide (fst (Ghost.reveal perm_map_pid))) in
-  let s = Seq.create (UInt32.v len) v in
-  (**) let h0 = HST.get() in
-  let content = HST.ralloc_mm HS.root s in
-  (**) let h1 = HST.get() in
-  (**) MG.modifies_ralloc_post #A.ucell #A.cls HS.root s h0 content h1;
-  let b = A.Array len content 0ul len (snd (Ghost.reveal perm_map_pid)) in
-  (**) assert (Seq.equal (A.as_seq h1 b) (Seq.create (UInt32.v len) init));
-  b
-
-let full_alloc (#a:Type) (init:a) (len:UInt32.t)
-  : RST (A.array a)
-        (empty_resource)
-        (fun b -> full_array_resource b)
-        (fun _ -> UInt32.v len > 0)
-        (fun _ b h1 ->
-        A.freeable b /\
-        (sel (array_view b) h1).s == Seq.create (UInt32.v len) init /\
-        (sel (array_view b) h1).p = FStar.Real.one
-        )
-  =   (**) reveal_array();
-  (**) reveal_rst_inv();
-  (**) reveal_modifies();
-  let b = arr_alloc init len in
-  // (**) let h1 = HST.get () in
-  // (**) assert(forall (i:nat{i < A.vlength #a b}). A.get_perm #a h1 b i = FStar.Real.one); // Find out how to trigger that
-  // (**) A.loc_includes_adresses_loc_array #a b true;
-  b
-
-let frame_full_pre (#a:Type) (b:A.array a) (res:resource) (pre:r_pre (array_resource b <*> res)) 
+let frame_full_pre (#a:Type) (b:A.array a) (res:resource) (pre:r_pre (array_resource b <*> res))
   (h:imem (inv (full_array_resource b <*> res)))
-  = 
+  =
+  reveal_full_array();
   reveal_array();
   reveal_star();
   pre h /\
   sel (array_view b) h == sel (full_array_view b) h
 
 let frame_full_post(#t:Type)
-                   (#a:Type) 
+                   (#a:Type)
                    (b:A.array a)
-                   (res0:resource) 
+                   (res0:resource)
                    (res1:t -> resource)
-                   (pre:r_pre (array_resource b <*> res0)) 
+                   (pre:r_pre (array_resource b <*> res0))
                    (post:r_post (array_resource b <*> res0) t (fun x -> array_resource b <*> res1 x))
                    (h0:imem (inv (full_array_resource b <*> res0)))
                    (x:t)
                    (h1:imem (inv (full_array_resource b <*> res1 x)))
     = reveal_array();
+      reveal_full_array();
       reveal_star();
       post h0 x h1 /\
       sel (array_view b) h1 == sel (full_array_view b) h1
@@ -267,7 +150,7 @@ let frame_full_array (#t:Type) (#a:Type) (b:A.array a)
     (res1:t -> resource)
     (#pre:r_pre (array_resource b <*> res0))
     (#post:r_post (array_resource b <*> res0) t (fun x -> array_resource b <*> res1 x))
-    ($f:unit -> RST t (array_resource b <*> res0) (fun x -> array_resource b <*> res1 x) pre post) 
+    ($f:unit -> RST t (array_resource b <*> res0) (fun x -> array_resource b <*> res1 x) pre post)
     : RST t
       (full_array_resource b <*> res0)
       (fun x -> full_array_resource b <*> res1 x)
